* Feeling really proud :)

Kleene.v
@@ -4,13 +4,13 @@ Import VectorNotations.
 
 Section to_be_moved.
 
-(** Random stuff about vectors to be placed elsewhere. *)
-Lemma hd_tl : forall {A} {n} (v:t A (S n)), v = hd v :: tl v.
-intros.
-revert n v; refine (@caseS _ _ _).
-simpl; auto.
+(** Random stuff about natural numbers. *)
+Lemma minus_S : forall n m, n - S m = pred (n - m).
+double induction n m; simpl; auto.
+intros; rewrite minus_n_O; auto.
 Qed.
 
+(** Random stuff about vectors to be placed elsewhere. *)
 Lemma eq_nth_iff' {A} {n} (v1 v2:t A n) : (forall (p:Fin.t n), v1[@p] = v2[@p]) <-> v1 = v2.
 split.
 intro; apply eq_nth_iff; intros; rewrite H0; auto.
@@ -50,11 +50,11 @@ End to_be_moved.
 Section Definitions.
 
 Inductive PRFunction : nat -> Set :=
-  | Zero : PRFunction 1
-  | Successor : PRFunction 1
-  | Projection : forall (m k:nat), k < m -> PRFunction m
-  | Composition : forall {k m:nat} (g:PRFunction m) (f:t (PRFunction k) m), PRFunction k
-  | Recursion : forall {k:nat} (g:PRFunction k) (h:PRFunction (2+k)), PRFunction (1+k)
+  | Zero         : PRFunction 1
+  | Successor    : PRFunction 1
+  | Projection   : forall {m k:nat}, k < m -> PRFunction m
+  | Composition  : forall {k m:nat} (g:PRFunction m) (fs:t (PRFunction k) m), PRFunction k
+  | Recursion    : forall {k:nat} (g:PRFunction k) (h:PRFunction (2+k)), PRFunction (1+k)
   | Minimization : forall {k:nat} (h:PRFunction (1+k)), PRFunction k
 .
 
@@ -88,7 +88,11 @@ Fixpoint eval_opt {m} (f:PRFunction m) : forall (steps:nat) (ns:t (option nat) m
 destruct f; intros.
 
 (* Zero *)
-+ apply (Some 0).
++ apply
+  match (nth ns (Fin.of_nat_lt (Nat.lt_succ_diag_r 0))) with
+    | Some x => Some 0
+    | None => None
+    end.
 
 (* Successor *)
 + apply
@@ -103,7 +107,7 @@ destruct f; intros.
 (* Composition *)
 + apply (eval_opt _ f).
   apply steps.
-  apply (map_inv (map_inv (map (eval_opt _) f0) steps) ns).
+  apply (map_inv (map_inv (map (eval_opt _) fs) steps) ns).
 
 (* Recursion *)
 + elim (hd ns); [idtac 1 | apply None].              (* is there an argument? *)
@@ -121,27 +125,6 @@ Defined.
 (* This is the one we actually want to use. *)
 Definition eval {m} (f:PRFunction m) (steps:nat) (ns:t nat m) : option nat := eval_opt f steps (map Some ns).
 
-(* Hmmm. *)
-Lemma eval_mon : forall m (f:PRFunction m) steps ns k, eval f steps ns = (Some k) ->
-  forall s', s' > steps -> eval f s' ns = (Some k).
-unfold eval.
-assert
-  (forall (m : nat) (f : PRFunction m) (steps : nat) (ns : t (option nat) m) (k : nat),
-    eval_opt f steps ns = Some k -> forall s' : nat, s' > steps -> eval_opt f s' ns = Some k).
-2: intros; apply H with steps; auto.
-induction f; intros.
-+ simpl; auto.
-+ simpl; auto.
-+ simpl; auto.
-+ simpl; simpl in H.
-  apply IHf with steps; auto.
-  replace (map_inv (map_inv (map eval_opt f0) s') ns) with (map_inv (map_inv (map eval_opt f0) steps) ns); auto.
-  apply eq_nth_iff'; intros.
-  repeat rewrite nth_map_inv'.
-  rewrite nth_map'.
-  Abort.
-
-
 End Definitions.
 
 Section Sanity_Checks.
@@ -157,7 +140,7 @@ replace (n+1) with (S n); auto.
 rewrite plus_comm; auto.
 Qed.
 
-Lemma Projection_correct : forall m k Hkm n steps, eval (Projection m k Hkm) steps n = Some (nth n (Fin.of_nat_lt Hkm)).
+Lemma Projection_correct : forall m k (Hkm: k<m) n steps, eval (Projection Hkm) steps n = Some (nth n (Fin.of_nat_lt Hkm)).
 intros; unfold eval; simpl.
 apply nth_map'.
 Qed.
@@ -201,25 +184,57 @@ simpl (map Some (x :: t)) in H0.
 simpl; simpl in H0; rewrite H0; auto.
 Qed.
 
+Lemma find_zero_from_correct : forall steps {k} f (ns:t (option nat) k) init m, find_zero_from f ns init steps = Some m ->
+  f ((Some m) :: ns) = Some O /\ forall n, init <= n < m -> exists val, f ((Some n) :: ns) = Some (S val).
+induction steps; intros.
++ inversion H.
++ revert H; simpl.
+  set (x := f (Some init :: ns)).
+  assert (x = f (Some init :: ns)); auto; clearbody x.
+  destruct x.
+  destruct n; intros.
+  - inversion H0; split.
+    * rewrite <- H2; auto.
+    * intros; elim (lt_irrefl m).
+      inversion_clear H1; apply le_lt_trans with n; auto.
+  - elim (IHsteps _ _ _ _ _ H0); intros; split; auto.
+    intros; inversion_clear H3.
+    elim (le_lt_eq_dec _ _ H4); intro.
+    * apply H2; auto with arith.
+    * exists n; rewrite <- b; auto.
+  - intro; inversion H0.
+Qed.
+
 Lemma Minimization_correct : forall k (h:PRFunction (1+k)) (ns:t nat k) steps n,
   eval (Minimization h) steps ns = (Some n) ->
-  eval h steps (n::ns) = (Some 0) /\ forall m, m < n -> exists n', eval h steps (n::ns) = (Some (S n')).
-Abort.
+  exists s, eval h s (n::ns) = (Some 0) /\ forall m, m < n -> exists n', eval h s (m::ns) = (Some (S n')).
+intros; revert H; unfold eval.
+induction steps.
++ simpl; intros; inversion H.
++ simpl; intro.
+  elim (find_zero_from_correct _ _ _ _ _ H); intros; exists steps; split; auto.
+  intros; apply H1; split; auto with arith.
+Qed.
 
 End Sanity_Checks.
 
 Section Examples.
 (** We recover the examples from the submitted journal paper. *)
 
-Lemma aux01 : 0 < 1.
+(* These lemmas are used to define projections. Their names seem inconsistent, but they refer to the usual convention for naming projections. *)
+Lemma aux11 : 0 < 1.
 auto with arith.
 Qed.
 
-Lemma aux13 : 1 < 3.
+Lemma aux13 : 0 < 3.
 auto with arith.
 Qed.
 
-Definition PR_add := Recursion (Projection 1 0 aux01) (Composition Successor [Projection 3 1 aux13]).
+Lemma aux23 : 1 < 3.
+auto with arith.
+Qed.
+
+Definition PR_add := Recursion (Projection aux11) (Composition Successor [Projection aux23]).
 
 Eval compute in (eval PR_add 0 [2; 3]).
 Eval compute in (eval PR_add 0 [5; 7]).
@@ -235,9 +250,9 @@ replace (m+n+1) with (S (m+n)); auto.
 rewrite (plus_comm (m+n) 1); auto with arith.
 Qed.
 
-Definition PR_sign := Composition (Recursion Zero
-  (Composition Successor [Composition Zero [Projection 3 1 aux13]]))
-  [Projection 1 0 aux01; Projection 1 0 aux01].
+Definition PR_sign := Composition
+  (Recursion Zero(Composition Successor [Composition Zero [Projection aux23]]))
+  [Projection aux11; Projection aux11].
 
 Eval compute in (eval PR_sign 0 [32]).
 Eval compute in (eval PR_sign 0 [0]).
@@ -246,13 +261,105 @@ Lemma sign_correct_0 : forall steps, eval PR_sign steps [0] = Some (0).
 intros; simpl; auto.
 Qed.
 
-Lemma sign_correct_S : forall m steps, eval PR_sign steps [S m] = Some (1).
-intros; induction m.
+Lemma sign_correct_S : forall n steps, eval PR_sign steps [S n] = Some (1).
+intros; induction n.
 simpl; auto.
 unfold PR_sign.
-revert IHm; unfold eval; simpl; intro.
-rewrite IHm; auto.
+revert IHn; unfold eval; simpl; intro.
+rewrite IHn; auto.
+Qed.
+
+Definition PR_pred := Composition (Recursion Zero (Projection aux13)) [Projection aux11; Zero].
+
+Eval compute in (eval PR_pred 0 [32]).
+Eval compute in (eval PR_pred 0 [0]).
+
+Lemma pred_correct : forall n steps, eval PR_pred steps [n] = Some (pred n).
+intros; unfold PR_pred.
+rewrite <- Composition_correct with (ms := [n; 0]).
++ induction n.
+  - rewrite Recursion_correct_base; auto.
+  - rewrite Recursion_correct_step with (x := n) (y := pred n); auto.
++ unfold eval; intro.
+  do 2 rewrite <- nth_map'.
+  repeat rewrite <- nth_map_inv'.
+  replace (map_inv (map_inv (map eval_opt [Projection aux11; Zero]) steps) (map Some [n])) with (map Some [n; 0]); auto.
+Qed.
+
+Definition PR_sub := Recursion (Projection aux11) (Composition PR_pred [Projection aux23]).
+
+Eval compute in (eval PR_sub 0 [2; 3]).
+Eval compute in (eval PR_sub 0 [5; 7]).
+Eval compute in (eval PR_sub 0 [3; 2]).
+
+Lemma sub_correct : forall m n steps, eval PR_sub steps [m; n] = Some (n - m).
+intros; unfold PR_sub.
+induction m.
++ rewrite Recursion_correct_base; auto; rewrite <- minus_n_O; auto.
++ rewrite Recursion_correct_step with (x := m) (y := n - m); simpl; auto.
+  replace (n - S m) with (pred (n - m)).
+  - rewrite <- Composition_correct with (ms := [n-m]).
+    * apply pred_correct.
+    * unfold eval; intro.
+      do 2 rewrite <- nth_map'.
+      do 2 rewrite <- nth_map_inv'.
+      replace (map_inv (map_inv (map eval_opt [Projection aux23]) steps) (map Some [m; n - m; n])) with (map Some [n-m]); auto.
+  - rewrite minus_S; auto.
 Qed.
 
 End Examples.
 
+(* Ongoing. *)
+
+Section Incomplete.
+
+Lemma eval_mon_comp : forall {k m:nat} (g:PRFunction m) (fs:t (PRFunction k) m) steps ns,
+  eval_opt (Composition g fs) steps ns = (Some k) ->
+  exists Hi, exists k', eval_opt fs[@Hi] steps ns = (Some k').
+intros.
+simpl in H.
+induction g; simpl in H.
++ repeat rewrite nth_map_inv' in H; rewrite nth_map' in H.
+  exists (Fin.F1 (n:=0)).
+  set (x := eval_opt fs[@Fin.F1] steps ns).
+  fold x in H.
+  induction x.
+  exists a; auto.
+  inversion H.
++ repeat rewrite nth_map_inv' in H; rewrite nth_map' in H.
+  exists (Fin.F1 (n:=0)).
+  set (x := eval_opt fs[@Fin.F1] steps ns).
+  fold x in H.
+  induction x.
+  exists a; auto.
+  inversion H.
++ repeat rewrite nth_map_inv' in H; rewrite nth_map' in H.
+  exists (Fin.of_nat_lt l).
+  set (x := eval_opt fs[@Fin.of_nat_lt l] steps ns).
+  fold x in H.
+  induction x.
+  exists a; auto.
+  inversion H.
++ Abort.
+
+(* Hmmm. *)
+Lemma eval_mon : forall m (f:PRFunction m) steps ns k, eval f steps ns = (Some k) ->
+  forall s', s' > steps -> eval f s' ns = (Some k).
+unfold eval.
+assert
+  (forall (m : nat) (f : PRFunction m) (steps : nat) (ns : t (option nat) m) (k : nat),
+    eval_opt f steps ns = Some k -> forall s' : nat, s' > steps -> eval_opt f s' ns = Some k).
+2: intros; apply H with steps; auto.
+induction f; intros.
++ simpl; auto.
++ simpl; auto.
++ simpl; auto.
++ simpl; simpl in H.
+  apply IHf with steps; auto.
+  replace (map_inv (map_inv (map eval_opt fs) s') ns) with (map_inv (map_inv (map eval_opt fs) steps) ns); auto.
+  apply eq_nth_iff'; intros.
+  repeat rewrite nth_map_inv'.
+  rewrite nth_map'.
+  Abort.
+
+End Incomplete.
